WIP in Asm lprsv

driver/IdSim.v
@@ -12,6 +12,10 @@ Require Import AxiomsC.
 Require Import Ord.
 Require Import MemoryC.
 Require Import SmallstepC.
+Require Import Events.
+Require Import Preservation.
+Require Import Integers.
+Require Import Locations Conventions.
 
 Set Implicit Arguments.
 
@@ -72,10 +76,9 @@ Qed.
 
 
 
-
-Local Existing Instance SimMemId.SimMemId | 0.
-Local Existing Instance SimMemId.SimSymbId | 0.
-Local Existing Instance SoundTop.Top | 0.
+(* Local Existing Instance SimMemId.SimMemId | 0. *)
+(* Local Existing Instance SimMemId.SimSymbId | 0. *)
+(* Local Existing Instance SoundTop.Top | 0. *)
 
 Lemma asm_id
       (asm: Asm.program)
@@ -100,44 +103,23 @@ Proof.
   ii; ss.
 
   exploit (SimSymbId.sim_skenv_revive PROG); try apply SIMSKENV; eauto.
-  (* hexploit (SimSymbId.sim_skenv_revive PROG). *)
   { i; ss. clarify. }
-  (* { instantiate (1:= (SkEnv.project skenv_link_src (defs asm))). eauto. } *)
-  (* { instantiate (1:= (SkEnv.project skenv_link_tgt (defs asm))). eauto. } *)
-  (* { ss. } *)
   intro GENV; des.
+  inv SIMSKENVLINK. inv SIMSKENV. ss.
 
   inv SIMARGS. destruct args_src, args_tgt; ss. clarify. destruct sm_arg; ss. clarify.
   fold fundef in *.
   split; ii; cycle 1.
-  { des. exists st_init_src. inv SAFESRC. econs; ss; eauto.
-    - unfold Genv.find_funct, Genv.find_funct_ptr in *. des_ifs_safe. inv GENV.
-      specialize (mge_defs b).
-      Local Opaque SkEnv.revive SkEnv.project.
-      unfold Genv.find_def in *. ss. rewrite Heq2 in *.
-      inv mge_defs; ss; clarify.
-      inv H1. ss.
-    - etrans; eauto.
-      admit "ez".
-  }
+  { des. exists st_init_src. inv SAFESRC. econs; ss; eauto. }
   rename tgt into m0.
   rename st_init_tgt into st0.
+  rename skenv_link_tgt into skenv_link.
   esplits; eauto.
-  { instantiate (1:= st0). clear SAFESRC.
-    inv INITTGT. econs; ss; eauto.
-    + unfold Genv.find_funct, Genv.find_funct_ptr in *. des_ifs_safe. inv GENV.
-      specialize (mge_defs b).
-      Local Opaque SkEnv.revive SkEnv.project.
-      unfold Genv.find_def in *. ss. rewrite Heq2 in *.
-      inv mge_defs; ss; clarify.
-      inv H1. ss.
-    + etrans; eauto. admit "ez".
-  }
   instantiate (1:= (SimMemId.mk m0 m0)). instantiate (1:= Ord.lift_idx unit_ord_wf tt).
   clear - GENV.
   generalize dependent st0.
   pcofix CIH. ii. pfold.
-  destruct (classic ((modsem skenv_link_src asm).(ModSem.is_call) st0)).
+  destruct (classic ((modsem skenv_link asm).(ModSem.is_call) st0)).
   { ss. rr in H. des.
     econs 3; eauto.
     { econs; eauto. }
@@ -145,18 +127,16 @@ Proof.
     exists args_src. exists (SimMemId.mk args_src.(Args.m) args_src.(Args.m)). ss.
     esplits; eauto.
     { econs; ss; eauto. }
-    { admit "ez". }
     ii. ss. des.
     esplits; eauto.
-    admit "ez".
+    inv SIMRETV. ss. destruct retv_src, retv_tgt; ss. clarify. destruct sm_ret; ss. clarify.
   }
-  destruct (classic ((modsem skenv_link_src asm).(ModSem.is_return) st0)).
+  destruct (classic ((modsem skenv_link asm).(ModSem.is_return) st0)).
   { ss. rr in H0. des.
     dup H0. set (R:= retv). inv H0.
     econs 4; eauto.
     { instantiate (1:= SimMemId.mk m2 m2). ss. }
     { econs; eauto. }
-    { ss. instantiate (1:= R). admit "ez". }
     { ss. }
   }
   econs 1; eauto.
@@ -167,7 +147,7 @@ Proof.
   ii. ss. inv STEPSRC.
   esplits; eauto. left. apply plus_one. econs; eauto.
   { admit "ez". }
-  econs; eauto. ss. admit "ez".
+  econs; eauto.
 Unshelve.
   all: ss.
 Qed.
@@ -184,6 +164,99 @@ Proof.
   admit "this should hold".
 Qed.
 
+Inductive sound_state (skenv: SkEnv.t) (su: Sound.t) (m_init: mem): AsmC.state -> Prop :=
+| sound_state_intro
+    init_rs rs0 m0
+    (MLE: Unreach.mle su m_init m0)
+    (RS: forall pr, UnreachC.val' su m0.(Mem.nextblock) (rs0#pr))
+    (MEM: UnreachC.mem' su m0)
+    (INIT: forall pr, UnreachC.val' su m0.(Mem.nextblock) (init_rs#pr))
+    (WF: forall blk (PRIV: su.(UnreachC.unreach) blk) (PUB: Plt blk su.(Unreach.ge_nb)), False)
+    (* (SKE: UnreachC.skenv su m0 skenv) *)
+    (SKE: su.(Unreach.ge_nb) = skenv.(Genv.genv_next))
+  :
+    sound_state skenv su m_init (mkstate init_rs (State rs0 m0))
+.
+
+Lemma val_nextblock
+      su0 blk0 blk1 v
+      (SU: UnreachC.val' su0 blk0 v)
+      (LE: Ple blk0 blk1)
+  :
+    <<SU: UnreachC.val' su0 blk1 v>>
+.
+Proof.
+  ii. clarify. exploit SU; eauto. i; des. esplits; eauto. xomega.
+Qed.
+
+Lemma asm_unreach_lprsv
+      asm skenv_link
+  :
+    exists sound_state,
+      <<PRSV: Preservation.local_preservation (modsem skenv_link asm) sound_state>>
+.
+Proof.
+  s.
+  exists (sound_state skenv_link).
+  econs; ii; ss; eauto.
+  - (* init *)
+    inv INIT. econs; eauto; ss.
+    + admit "this is nontrivial - this may be false, we should adjust it
+(we are not using Mem.store, but just quantifying. There may be unquantified memory area.)".
+    + admit "this should hold: TODO: fix PTRFREE".
+    + rr in SUARG. des; ss.
+      admit "this should hold".
+    + admit "this should hold: TODO: fix PTRFREE".
+    + inv SUARG. des. ss.
+    + inv SKENV. rewrite PUB in *. ss.
+  - (* step *)
+      admit "ez".
+  - (* call *)
+    inv AT. ss.
+    exploit (Sound.greatest_ex su0 (Args.mk (Vptr blk0 Ptrofs.zero true) vs m1)); ss; eauto.
+    { exists su0. esplits; eauto.
+      { refl. }
+      inv SUST. econs; ss; eauto.
+      + ii. exploit (RS PC); eauto. i; des. clarify. esplits; eauto. admit "ez".
+      + esplits; eauto.
+        * rewrite Forall_forall. i.
+          admit "extcall-arguments".
+        * admit "this should hold".
+    }
+    esplits; eauto.
+    + inv SUST.
+      etrans; eauto.
+      exploit RS; eauto. intro SU; des.
+      eapply Unreach.free_mle; eauto.
+    + admit "somehow... this should have been proven in somewhere else".
+    + ii. inv AFTER. ss.
+      destruct retv; ss. rename m into m2.
+      econs; eauto.
+      { inv SUST. etrans; eauto.
+        admit "free-mle-unfree dual".
+      }
+      { admit "this should hold". }
+      { inv SUST. admit "nontrivial... free-mle-unfree". }
+      { inv SUST.
+        ii. exploit INIT; eauto. i; des. esplits; eauto. admit "ez".
+      }
+      { inv SUST. ss. }
+      { inv SUST. ss. }
+  - (* return *)
+    inv SUST. inv FINAL. ss. clarify.
+    exists su0. esplits; eauto.
+    { refl. }
+    { econs; ss.
+      - erewrite Mem.nextblock_free; eauto.
+      - admit "this should hold".
+    }
+    etrans; eauto.
+    eapply UnreachC.free_mle; eauto.
+    exploit INIT; eauto. i; des. ss.
+Unshelve.
+  all: ss.
+Qed.
+
 Lemma asm_ext_unreach
       (asm: Asm.program)
   :
@@ -193,6 +266,29 @@ Lemma asm_ext_unreach
       /\ (<<TGT: mp.(ModPair.tgt) = asm.(AsmC.module)>>)
 .
 Proof.
+  eexists (ModPair.mk _ _ _); s.
+  assert(PROGSKEL: match_program (fun _ => eq) eq (Sk.of_program fn_sig asm) (Sk.of_program fn_sig asm)).
+  { econs; eauto. ss. eapply match_program_refl; eauto. }
+  assert(PROG: match_program (fun _ => eq) eq asm asm).
+  { econs; eauto. ss. eapply match_program_refl; eauto. }
+  esplits; eauto.
+  econs; ss; eauto.
+  ii. inv SSLE. clear_tac.
+
+  econs; ss; eauto.
+  { eapply SoundTop.sound_state_local_preservation; eauto. }
+  ii; ss.
+
+  exploit (SimSymbId.sim_skenv_revive PROG); try apply SIMSKENV; eauto.
+  { i; ss. clarify. }
+  intro GENV; des.
+  inv SIMSKENVLINK. inv SIMSKENV. ss.
+
+  inv SIMARGS. destruct args_src, args_tgt; ss. clarify. destruct sm_arg; ss. clarify.
+  fold fundef in *.
+  split; ii; cycle 1.
+  { des. exists st_init_src. inv SAFESRC. econs; ss; eauto. }
+  rename tgt into m0.
   admit "this should hold".
 Qed.
 
